---
title: Homework - Week 11
author: Adam Collado
toc: true
block-headings: true
---
\newpage

## Question 5

### a) Prove for any positive integer $n$, 3 divide $n^3 + 2n$

__Theorem:__ For any positive integer $n$, 3 divide $n^3 + 2n$

__Base Case:__ n = 1

P(1) is true due to the following:

$$
P(1) = n^3 + 2n = 1^3 + 2(1) = 1 + 2 = 3
$$

3 divides 3, thus P(1) is shown to be true.

__Inductive Step:__ We will show that when P(k) is true for any positive integer $k$, 3 divide $k^3 + 2k$, it follows that P(k+1), the statement 3 divide $(k+1)^3 + 2(k+1)$ is also true.

This can be shown with the following:

$$
\begin{aligned}
    P(k+1) &= (k+1)^3 + 2(k+1) \\
    &=k^3 + 3k^2 + 3k + 1 + 2k + 2 & \text{by algebra} \\
    &=k^3 + 3k + 3k^2 + 3k + 3
\end{aligned}
$$

Using the inductive hypothesis, we can conclude that 3 divides the term $k^3 + 3k$. We can also see that the reminder of the term, $3k^2 + 3k + 3$, can also be divided by 3.

Therefore, 3 divide $(k+1)^3 + 2(k+1)$
$\blacksquare$

### b) Use strong induction to prove that any positive integer $n(n \geq 2)$ can be written as a product of primes. 

\newpage

## Question 6

### 7.4.1: Components of an inductive proof.

Define P(n) to be the assertion that:

$$
\sum_{j=1}^{n}j^2 = \frac{n(n+1)(2n+1)}{6}
$$

#### a) Verify that P(3) is true.

__Solution:__ The equation is proof showing how to ge the sum of squares for numbers 1 to n. If this is so, then P(3) should calculate to:

$$
1^2 + 2^2 + 3^2 = 14
$$

And we can see after calculating for P(3):

$$
P(3) = \frac{n(n+1)(2n+1)}{6} = \frac{3(3+1)(2(3)+1)}{6} = \frac{3(4)(7)}{6} = \frac{84}{6} = 14
$$

Thus, P(3) = 14, and therefore proves true.

#### b) Express P(k).

__Solution:__

$$
P(k) = \frac{k(k+1)(2k+1)}{6}
$$

#### c) Express P(K + 1).

__Solution:__:

$$
P(k + 1) = \frac{(k+1)(k+2)(2k+3)}{6}
$$

#### d) In the inductive proof that for every positive integer n, what must be proven in the base case?

The base case must prove that the theorem is true for the first value of the sequence. In the case of this theorem our base case would be P(1), since the equation states that j=1 to n.

#### e) In an inductive proof that for every positive integer n, what must be proven in the inductive step?

The inductive step must prove that if the theorem holds for P(k) (which is assume to be true), then it holds true that P(k + 1).


#### f) What would be the inductive hypothesis in the inductive step from your previous answer?

The inductive hypothesis would be the statement P(k) being true.

#### g) Prove by induction that for any positive n.

First we will prove the base case that was stated in part d of this question.

__Base Case:__ $n = 1$

$$
P(1) = 1^2 = \frac{n(n+1)(2n+1)}{6} = \frac{(1+1)(2+1)}{6} = \frac{(2)(3)}{6} = \frac{6}{6} = 1
$$

Therefore, $\sum_{j=1}^{1} j^2 = \frac{1(1 + 1)(2(1) + 1)}{6}$

__Inductive Step:__  Suppose that for a positive integer $k$:

$$
\sum_{j=1}^{k} j^2 \frac{k(k+1)(2k+1)}{6}
$$

We will show that for when $P(k+1)$:

$$
\sum_{j=1}^{k+1} j^2 \frac{(k+1)(k+2)(2k+3)}{6}
$$

We will start with the left side of the equation and continue:

$$
\begin{aligned}
    \sum_{j=1}^{k+1} j^2 &= \sum_{j=1}^{k} + (k + 1)^2 & \text{separating the last }\\
    &= \frac{k(k+1)(2k+1)}{6} + (k + 1)^2 & \text{by inductive step}\\
    &= \frac{k(k+1)(2k+1) + 6(k+1)^2}{6} & \\
    &= \frac{k(k+1)(2k+1) + 6(k+1)(k+1)}{6} & \\
    &= \frac{(k+1)(k(2k+1) + 6(k+1))}{6} & \text {by algebra} \\
    &= \frac{(k+1)(2k^2+k + 6k+6)}{6} & \\ 
    &= \frac{(k+1)(k+2)(2k+3)}{6} & \\ 
\end{aligned}
$$

Therefore, $\sum_{j=1}^{k+1} j^2 \frac{(k+1)(k+2)(2k+3)}{6}$
$\blacksquare$

### 7.4.3

Prove each of the following statements using mathematical induction.

#### c)

__Theroem:__ For any positive integer n, $\sum_{j=1}^{n} \frac{1}{j^2} \leq 2 - \frac{1}{n}$

__Base Case:__ n = 1

We can show the following:

$$
\frac{1}{1^2} = 1 \leq 2 - \frac{1}{1} = 1
$$

Thus proving P(1)

__Inductive Step__: We will show that when P(k) is true for any positive integer k, $\sum_{j=1}^{k} \frac{1}{j^2} \leq 2 - \frac{1}{k}$, it follow that P(k+1), $\sum_{j=1}^{k+1} \frac{1}{j^2} \leq 2 - \frac{1}{k+1}$ will also hold true.

We will show this with the following:

$$
\begin{aligned}
    \sum_{j=1}^{k+1}\frac{1}{j^2} &= \sum_{j=1}^{k}\frac{1}{j^2} + \frac{1}{(k+1)^2} \\
    &\leq 2 - \frac{1}{k} + \frac{1}{(k+1)^2} & \text{by inductive hypothesis} \\
    &\leq 2 - \frac{1}{k} + \frac{1}{k(k+1)} & \text{by algebra} \\
    &= 2 -\frac{k+1}{k(k+1)} + \frac{1}{k(k+1)} \\
    &= 2 - \frac{k}{k(k+1)} \\
    &= 2 - \frac{1}{k+1} 

\end{aligned}
$$

Therefore, $\sum_{j=1}^{k+1} \frac{1}{j^2} \leq 2 - \frac{1}{k+1}$
$\blacksquare$

### 7.5.1

#### a)